updated coq formalization

proofs/core/basics.v
@@ -6,6 +6,24 @@ Require Import Coq.Lists.List.
 Require Import Coq.Classes.EquivDec.
 
 
+Inductive styp :=
+  | Sint : styp
+  | Stop : styp
+  | Sarr : styp -> styp -> styp
+  | Sand : styp -> styp -> styp
+  | Srcd : string -> styp -> styp
+  | Ssig : styp -> styp -> styp.
+
+Inductive sop := Sapp.
+
+Inductive sexp :=
+  | Sctx        : sexp  
+  | Sunit       : sexp
+  | Slit        : nat   -> sexp
+  | Sbinop      : sop   -> sexp -> sexp -> sexp
+  | Slam        : styp  -> sexp -> sexp.
+
+
 Inductive typ :=
   | int : typ
   | top : typ
@@ -13,18 +31,56 @@ Inductive typ :=
   | and : typ -> typ -> typ
   | rcd : string -> typ -> typ.
 
-Inductive op := app | mrg.
+Inductive elaborate_typ : styp -> typ -> Prop :=
+  | elint : elaborate_typ Sint int
+  | eltop : elaborate_typ Stop top
+  | elarr : forall A A' B B',
+            elaborate_typ A A' ->
+            elaborate_typ B B' ->
+            elaborate_typ (Sarr A B) (arr A' B')
+  | eland : forall A A' B B',
+            elaborate_typ A A' ->
+            elaborate_typ B B' ->
+            elaborate_typ (Sand A B) (and A' B')
+  | elrcd : forall l A A',
+            elaborate_typ A A' ->
+            elaborate_typ (Srcd l A) (rcd l A')
+  | elsig : forall A A' B B',
+            elaborate_typ A A' ->
+            elaborate_typ B B' ->
+            elaborate_typ (Ssig A B) (arr A' B').
+
+Inductive op := app | box | mrg.
 
 Inductive exp :=
   | ctx         : exp
   | lit         : nat -> exp
   | unit        : exp
   | binop       : op -> exp -> exp -> exp
+  | lam         : typ -> exp -> exp
   | proj        : exp -> nat -> exp
   | clos        : exp -> typ -> exp -> exp
   | rec         : string -> exp -> exp
   | rproj       : exp -> string -> exp.
 
+Inductive elaborate_sexp : styp -> sexp -> styp -> exp -> Prop :=
+  | infctx: forall E, 
+        elaborate_sexp E Sctx E ctx
+  | infint: forall E n,
+        elaborate_sexp E (Slit n) Sint (lit n)
+  | infunit: forall E,
+        elaborate_sexp E Sunit Stop unit
+  | inflam: forall E A A' Se e B,
+      elaborate_typ A A' ->
+      elaborate_sexp (Sand E A) Se B e ->
+      elaborate_sexp E (Slam A Se) (Sarr A B) (lam A' e)
+(*  | tapp : forall E A B e1 e2,
+      has_type E e1 (arr A B) -> has_type E e2 A -> has_type E (binop app e1 e2) B *)
+  | infapp: forall E A B sE1 sE2 cE1 cE2,
+      elaborate_sexp E sE2 A cE2 ->
+      elaborate_sexp E sE1 (Sarr A B) cE1 ->
+      elaborate_sexp E (Sbinop Sapp sE1 sE2) B (binop app cE1 cE2).
+  
 Inductive lookup : typ -> nat -> typ -> Prop :=
   | lzero : forall A B, 
       lookup (and A B) 0 B
@@ -65,19 +121,20 @@ Inductive has_type : typ -> exp -> typ -> Prop :=
   | tint : forall E i, has_type E (lit i) int
   | tunit : forall E, has_type E unit top
   | tapp : forall E A B e1 e2,
-      has_type E e1 (arr A B) ->
-      has_type E e2 A ->
-      has_type E (binop app e1 e2) B
+      has_type E e1 (arr A B) -> has_type E e2 A -> has_type E (binop app e1 e2) B
+  | tbox : forall E A E1 e1 e2,
+      has_type E e1 E1 -> has_type E1 e2 A -> has_type E (binop box e1 e2) A
   | tmrg : forall E e1 e2 A B,
-      has_type E e1 A -> 
-      has_type (and E A) e2 B ->
-      has_type E (binop mrg e1 e2) (and A B)
+      has_type E e1 A -> has_type (and E A) e2 B -> has_type E (binop mrg e1 e2) (and A B)
+  | tlam : forall E A e B,
+      has_type (and E A) e B -> has_type E (lam A e) (arr A B)
   | tproj: forall E A e B n,
       has_type E e A ->
       lookup A n B ->
       has_type E (proj e n) B
-  | tclos : forall E E1 A e ev B,
-      has_type top ev E1 ->
+  | tclos : forall E E1 A e ev B, 
+      value ev ->
+      has_type top ev E1 -> 
       has_type (and E1 A) e B -> 
       has_type E (clos ev A e) (arr A B)
   | trcd : forall E e A l,
@@ -118,22 +175,29 @@ Inductive step : exp -> exp -> exp -> Prop :=
       value v1 -> 
       step v e2 e2' -> 
       step v (binop app v1 e2) (binop app v1 e2')
+  | sbbox : forall v v1 e2 e2', 
+      value v -> 
+      value v1 -> 
+      step v1 e2 e2' -> 
+      step v (binop box v1 e2) (binop box v1 e2')
   | sbmrg : forall v v1 e' e,
-      value v ->
-      value v1 ->
+      value v -> 
+      value v1 -> 
       step (binop mrg v v1) e e' -> 
       step v (binop mrg v1 e) (binop mrg v1 e')
-  | sbeta : forall v v1 v2 A e e', 
-      value v   -> 
-      value v1  -> 
-      value v2 ->
-      step (binop mrg v2 v1) e e' ->
-      step v (binop app (clos v2 A e) v1) (binop app (clos (binop mrg v2 v1) top e') unit)
-  | sbetav : forall v v1 v2,
+  | sclos : forall v A e, 
+      value v -> 
+      step v (lam A e) (clos v A e)
+  | sbeta : forall v v1 v2 A e, 
+      value v -> 
+      value v1 ->
+      value v2 -> 
+      step v (binop app (clos v2 A e) v1) (binop box (binop mrg v2 v1) e)
+  | sboxv : forall v v1 v2,
       value v -> 
       value v1 -> 
       value v2 -> 
-      step v (binop app (clos v1 top v2) unit) v2
+      step v (binop box v1 v2) v2
   | sproj: forall v e1 e2 n,
       value v ->
       step v e1 e2 ->
@@ -157,333 +221,43 @@ Inductive step : exp -> exp -> exp -> Prop :=
       rlookupv v1 l v2 ->
       step v (rproj v1 l) v2.
 
-
 #[export]
-Hint Constructors typ op exp lookup lookupv lin rlookup has_type value rlookupv step : core.
+Hint Constructors typ op exp lookup lookupv lin rlookup styp sop sexp elaborate_typ elaborate_sexp has_type value rlookupv step : core.
 
 
 Require Import Program.Equality.
 
+Lemma type_elaboration_unique : forall E E' E'',
+  elaborate_typ E E' ->
+  elaborate_typ E E'' ->
+  E' = E''.
+Proof.
+  intros E E' E'' H1 H2.
+  generalize dependent E''.
+  induction H1; intros E'' H2; try inversion H2; subst; try reflexivity;
+    try ( apply IHelaborate_typ1 in H1;
+          apply IHelaborate_typ2 in H4;
+          rewrite H1; rewrite H4; reflexivity).
+  + apply IHelaborate_typ in H4.
+    rewrite H4. reflexivity.
+Qed.
 
-(* Type soundness *)
-Lemma value_weaken : forall E v A,
-  has_type E v A -> forall E',
-  value v ->
-  has_type E' v A.
-Proof. 
-  intros E v A H.
-  induction H;
-  intros E' Hv.
-  + inversion Hv.
-  + apply tint. 
+(* ---------------------------------------------------- *)
+(* Elaboration *)
+Lemma type_safe_translation : forall E E' SE A A' CE,
+  elaborate_typ E E' ->
+  elaborate_typ A A' ->
+  elaborate_sexp E SE A CE ->
+  has_type E' CE A'.
+Proof.
+  intros E E' SE A A' CE HA HE H.
+  generalize dependent A'.
+  generalize dependent E'.
+  induction H.
+  
+  induction H; subst; exists; intros HE HA.
+  + apply tctx.
+  + apply tint.
   + apply tunit.
-  + inversion Hv.
-  + inversion Hv; subst.
-    - apply tmrg.
-      ++ apply IHhas_type1. assumption.
-      ++ apply IHhas_type2. assumption.
-  + inversion Hv.
-  + inversion Hv; subst.
-    apply tclos with (E1 := E1); assumption.
-  + inversion Hv; subst. apply trcd. apply IHhas_type. assumption.
-  + inversion Hv.
+  + apply tlam.
 Qed.
-
-
-Lemma lookupv_value: forall v n v',
-  lookupv v n v' ->
-  value v        ->
-  value v'.
-Proof.
-  introv Hl.
-  induction Hl; intros Hv.
-  + inversion Hv; assumption.
-  + inversion Hv; subst. apply IHHl. assumption.
-Qed.
-
-Lemma lookup_pres_ctx: forall E n A,
-  lookup E n A -> forall v v',
-  lookupv v n v' -> 
-  value v ->
-  has_type top v E ->
-  has_type E v' A.
-Proof.
-  introv Hl. inductions Hl; introv Hlv Hv Ht.
-  - inverts* Hlv. inverts* Ht. inverts Hv.
-    eapply value_weaken; eauto.
-  - inverts* Hlv. inverts* Ht. inverts Hv.
-    forwards~: IHHl H1 H2.
-    eapply value_weaken; eauto.
-    eapply lookupv_value; eauto.
-Qed.
-
-Lemma lookup_pres: forall E n A,
-  lookup E n A -> forall v v',
-  lookupv v n v' -> 
-  value v ->
-  has_type top v E ->
-  has_type top v' A.
-Proof.
-  introv Hl Hlv Hv Ht.
-  forwards~: lookup_pres_ctx Hl Hlv Hv Ht.
-  eapply value_weaken; eauto.
-  eapply lookupv_value; eauto. 
-Qed.
-
-
-Lemma rlookupv_value: forall v l v', 
-  rlookupv v l v' -> 
-  value v -> 
-  value v'.
-Proof.
-  introv Hl. inductions Hl; introv Hv; inverts* Hv.
-Qed.
-
-
-Lemma rcd_shape: forall E v l B, 
-  has_type E v (rcd l B) -> 
-  value v -> exists v',
-  v = rec l v'.
-Proof.
-  introv Ht. inductions Ht; introv Hv;
-  try solve [inverts* Hv].
-Qed. 
-
-Lemma notin_false: forall E v A,
-  has_type E v A -> forall l v',
-  rlookupv v l v' ->
-  ~ lin l A ->
-  False.
-Proof.
-  introv Ht. inductions Ht; introv Hr Hnl;
-  try solve [inverts* Hr].
-Qed.
-
-Lemma rlookup_pres_aux: forall E l A,
-  rlookup E l A -> forall v v',
-  rlookupv v l v' -> 
-  value v ->
-  has_type top v E ->
-  has_type E v' A.
-Proof.
-  introv Hl. inductions Hl; introv Hlv Hv Ht.
-  - inverts* Ht; try solve [inverts Hv].
-    inverts Hlv. inverts Hv.
-    eapply value_weaken; eauto.
-  - inverts* Hlv; try solve [inverts* Ht]. 
-    + inverts Ht. inverts Hv.
-      forwards~: IHHl H0 H5. 
-      eapply value_weaken; eauto.
-      eapply rlookupv_value; eauto.
-    + inverts Ht. inverts Hv. 
-      exfalso. eapply notin_false; eauto.
-  - inverts* Hlv; try solve [inverts* Ht]. 
-    + inverts Ht. inverts Hv. 
-      exfalso. eapply notin_false; try eapply H; eauto.
-    + inverts Ht. inverts Hv.
-      forwards~: IHHl H0. 
-      eapply value_weaken; eauto.
-      eapply value_weaken; eauto.
-      eapply rlookupv_value; eauto.
-Qed. 
-
-Lemma rlookup_pres: forall E l A,
-  rlookup E l A -> forall v v',
-  rlookupv v l v' -> 
-  value v ->
-  has_type top v E ->
-  has_type top v' A.
-Proof.
-  introv Hl Hlv Hv Ht.
-  forwards~: rlookup_pres_aux Hl Hlv Hv Ht.
-  eapply value_weaken; eauto.
-  eapply rlookupv_value; eauto.
-Qed.
-
-(* 
-  7 goals
-  v : exp
-  H : value v
-  E, A : typ
-  Ht : has_type E ctx A
-  Htv : has_type top v E
-  ______________________________________(1/7)
-  has_type E v A
-  ______________________________________(2/7)
-  has_type E (binop box v1 e2') A
-  ______________________________________(3/7)
-  has_type E (binop mrg v1 e') A
-  ______________________________________(4/7)
-  has_type E (binop box (binop mrg v2 v1) e) A0
-  ______________________________________(5/7)
-  has_type E v2 A
-  ______________________________________(6/7)
-  has_type E v2 A
-  ______________________________________(7/7)
-  has_type E v2 A
-
-*)
-Definition useful : forall A e B,
-    has_type A e B ->
-    has_type (and A top) e B.
-Proof.
-Admitted.
-
-Definition useful2 : forall A e B,
-  has_type A e B ->
-  has_type A e (and B top).
-Admitted.
-
-Lemma gpreservation : forall e e' v, 
-  step v e e' -> forall E A, 
-  has_type E e A -> 
-  has_type top v E -> 
-  has_type E e' A.
-Proof.
-  introv Hs. inductions Hs; introv Ht Htv;
-  try solve [eauto];
-  try solve [inverts* Ht].
-  - inversion Ht; subst.
-    apply value_weaken with (E := top); assumption.
-  - inverts* Ht.
-    econstructor; eauto.
-    eapply IHHs; eauto.
-    econstructor; eauto.
-    eapply value_weaken; eauto.
-  - inversion Ht; subst.
-    inversion H5; subst.
-    apply tapp with (A := top).
-    + apply tclos with (E1 := and E1 A1).
-
-
-
-inversion Ht; subst.
-    apply tapp with (A
-    + 
-    apply tclos with (E1 := and A1 A1).
-      -- apply tmrg; eauto using value_weaken.
-      ++ apply IHHs.
-
-  - inverts* Ht.
-    forwards~: lookup_pres H7 H1.
-    eapply value_weaken; eauto.
-    eapply value_weaken; eauto.
-    eapply lookupv_value; eauto.
-  - inverts* Ht.
-    forwards~: rlookup_pres H7 H1.
-    eapply value_weaken; eauto.
-    eapply value_weaken; eauto.
-    eapply rlookupv_value; eauto.
-Qed.
-
-Lemma lookup_prog: forall n A B,
-  lookup A n B -> forall v,
-  has_type top v A ->
-  value v ->
-  exists e', lookupv v n e'.
-Proof.
-  introv Hl. inductions Hl; introv Ht Hv.
-  - inverts* Ht; try solve [inverts* Hv].
-  - inverts* Ht; try solve [inverts* Hv].
-    + inverts* Hv. 
-      forwards~ (e'&Hs): IHHl H3.
-      inverts* Hs.
-Qed.
-
-Lemma rlookup_prog: forall n A B,
-  rlookup A n B -> forall v,
-  has_type top v A ->
-  value v ->
-  exists e', rlookupv v n e'.
-Proof.
-  introv Hl. inductions Hl; introv Ht Hv.
-  - inverts* Ht; try solve [inverts* Hv].
-  - inverts* Ht; try solve [inverts* Hv].
-    inverts Hv.
-    forwards~ (?&?): IHHl H4.
-    exists* x.
-  - inverts* Ht; try solve [inverts* Hv].
-    inverts Hv.
-    forwards~ (?&?): IHHl e2.
-    eapply value_weaken; eauto.
-    exists* x.
-Qed.
-
-
-Lemma gprogress : forall E e A, 
-  has_type E e A -> forall v, 
-  value v -> 
-  has_type top v E -> 
-  value e \/ exists e', step v e e'.
-Proof.
-  introv Ht.
-  inductions Ht; introv Hv Htv; eauto.
-  - right.
-    forwards~: IHHt1 Htv.
-    forwards~: IHHt2 Htv.
-    destruct* H; destruct* H0.
-    + inverts* Ht1; inverts* H.
-    + inverts* H0.
-    + inverts* H.
-    + inverts* H.
-  - forwards~: IHHt1 Htv.
-    destruct H.
-    + forwards~: IHHt2 H.
-      eapply value_weaken; eauto.
-      destruct* H0. right*. inverts* H0.
-    + inverts* H.
-  - forwards~: IHHt1 Htv.
-    destruct H.
-    + forwards~: IHHt2 (binop mrg v e1).
-      econstructor; eauto.
-      eapply value_weaken; eauto.
-      destruct* H0.
-      destruct* H0.
-    + inverts* H.
-  - right.
-    forwards~: IHHt Hv.
-    inverts H0.
-    + forwards~: value_weaken Ht top.
-      forwards~ (?&?): lookup_prog H H0.
-      exists* x.
-    + inverts* H1.
-  - forwards~: IHHt Hv Htv. destruct* H.
-    right*. destruct* H. 
-  - right.
-    forwards~: IHHt Hv.
-    inverts H0.
-    + forwards~: value_weaken Ht top.
-      forwards~ (?&?): rlookup_prog H H0.
-      exists* x. 
-    + inverts* H1.
-Qed.
-
-Lemma preservation : forall e e' A, has_type top e A -> step unit e e' -> has_type top e' A.
-  intros.
-  eapply gpreservation; eauto.
-Defined.
-      
-Lemma progress :  forall e A, has_type top e A -> value e \/ exists e', step unit e e'.
-  intros.
-  eapply gprogress; eauto.
-Defined.
-
-
-
-
-
-
-
-
-
-
-
-
-
-
-
-
-
-
-
-
